src/concurrency/DNS.Worker.Minimal.fst
@@ -7,6 +7,12 @@ open Steel.Memory
 open Steel.ST.Util
 open DNS.QUIC.StreamMapping
 
+let noerror_response_flags_hi (request_flags_hi:FStar.UInt8.t) : FStar.UInt8.t =
+  FStar.UInt8.logor 0x80uy (FStar.UInt8.logand request_flags_hi 0x79uy)
+
+let noerror_response_flags_lo (request_flags_lo:FStar.UInt8.t) : FStar.UInt8.t =
+  FStar.UInt8.logand request_flags_lo 0x10uy
+
 val prepare_worker_minimal_error_response_send :
   ctx_ptr:buffer stream_context ->
   response_buffer:buffer FStar.UInt8.t ->
@@ -57,6 +63,69 @@ let prepare_worker_minimal_error_response_send
       LowStar.Buffer.upd response_buffer 1ul id_lo;
       LowStar.Buffer.upd response_buffer 2ul 0x81uy;
       LowStar.Buffer.upd response_buffer 3ul 0x03uy;
+      LowStar.Buffer.upd response_buffer 4ul 0x00uy;
+      LowStar.Buffer.upd response_buffer 5ul 0x00uy;
+      LowStar.Buffer.upd response_buffer 6ul 0x00uy;
+      LowStar.Buffer.upd response_buffer 7ul 0x00uy;
+      LowStar.Buffer.upd response_buffer 8ul 0x00uy;
+      LowStar.Buffer.upd response_buffer 9ul 0x00uy;
+      LowStar.Buffer.upd response_buffer 10ul 0x00uy;
+      LowStar.Buffer.upd response_buffer 11ul 0x00uy;
+      12ul
+    end
+
+val prepare_worker_empty_noerror_response_send :
+  ctx_ptr:buffer stream_context ->
+  response_buffer:buffer FStar.UInt8.t ->
+  response_capacity:FStar.UInt32.t ->
+  request_len:FStar.UInt32.t ->
+  ST FStar.UInt32.t
+    (requires (fun h0 ->
+      live h0 ctx_ptr /\
+      LowStar.Buffer.length ctx_ptr >= 1 /\
+      live h0 response_buffer /\
+      FStar.UInt32.v response_capacity <= LowStar.Buffer.length response_buffer /\
+      (let ctx = FStar.Seq.index (LowStar.Buffer.as_seq h0 ctx_ptr) 0 in
+       live h0 ctx.sc_buf /\
+       FStar.UInt32.v request_len <= LowStar.Buffer.length ctx.sc_buf)))
+    (ensures (fun h0 _ h1 ->
+      modifies (loc_buffer response_buffer) h0 h1 /\
+      live h1 response_buffer))
+
+let prepare_worker_empty_noerror_response_send
+  ctx_ptr
+  response_buffer
+  response_capacity
+  request_len =
+  let s = LowStar.Buffer.index ctx_ptr 0ul in
+  if FStar.UInt32.lt request_len 12ul ||
+     FStar.UInt32.lt response_capacity 12ul then
+    0ul
+  else
+    begin
+      assert (FStar.UInt32.v request_len <= LowStar.Buffer.length s.sc_buf);
+      assert (12 <= LowStar.Buffer.length response_buffer);
+      assert (3 < LowStar.Buffer.length s.sc_buf);
+      assert (0 < LowStar.Buffer.length response_buffer);
+      assert (1 < LowStar.Buffer.length response_buffer);
+      assert (2 < LowStar.Buffer.length response_buffer);
+      assert (3 < LowStar.Buffer.length response_buffer);
+      assert (4 < LowStar.Buffer.length response_buffer);
+      assert (5 < LowStar.Buffer.length response_buffer);
+      assert (6 < LowStar.Buffer.length response_buffer);
+      assert (7 < LowStar.Buffer.length response_buffer);
+      assert (8 < LowStar.Buffer.length response_buffer);
+      assert (9 < LowStar.Buffer.length response_buffer);
+      assert (10 < LowStar.Buffer.length response_buffer);
+      assert (11 < LowStar.Buffer.length response_buffer);
+      let id_hi = LowStar.Buffer.index s.sc_buf 0ul in
+      let id_lo = LowStar.Buffer.index s.sc_buf 1ul in
+      let request_flags_hi = LowStar.Buffer.index s.sc_buf 2ul in
+      let request_flags_lo = LowStar.Buffer.index s.sc_buf 3ul in
+      LowStar.Buffer.upd response_buffer 0ul id_hi;
+      LowStar.Buffer.upd response_buffer 1ul id_lo;
+      LowStar.Buffer.upd response_buffer 2ul (noerror_response_flags_hi request_flags_hi);
+      LowStar.Buffer.upd response_buffer 3ul (noerror_response_flags_lo request_flags_lo);
       LowStar.Buffer.upd response_buffer 4ul 0x00uy;
       LowStar.Buffer.upd response_buffer 5ul 0x00uy;
       LowStar.Buffer.upd response_buffer 6ul 0x00uy;
